src/lib/kernel/gemm/Kuiper.Kernel.GEMM.TensorCore2D.To.Epilogue.fst
@@ -4,7 +4,7 @@ module Kuiper.Kernel.GEMM.TensorCore2D.To.Epilogue
 
 open Kuiper
 #set-options "--ifuel 1 --initial_fuel 0 --max_fuel 1"
-#set-options "--z3rlimit 120"
+#set-options "--z3rlimit 15"
 
 open Kuiper.Array.Vectorized { has_vec_cpy, chunk }
 open Kuiper.EMatrix
@@ -22,184 +22,12 @@ open Pulse.Lib.Array
 open Pulse.Lib.Trade
 
 module SZ = Kuiper.SizeT
-module T = Kuiper.Tensor
-module CV2 = Kuiper.Kernel.GEMM.Copy.Vec2
 
 open Kuiper.Kernel.GEMM.TensorCore2D.KernelDesc
 open Kuiper.Kernel.GEMM.TensorCore2D.To.KernelDesc
-
-let output_fragment_post
-  (#et : Type0) {| scalar et, real_like et |}
-  (#m #n : nat)
-  (gD : array2 et (rm m n))
-  (bm bn tm tn wm wn : pos)
-  (#_ : squash (bm /?+ m /\ bn /?+ n /\
-                wm * tm /?+ bm /\ wn * tn /?+ bn))
-  (bid : natlt (m / bm * (n / bn)))
-  (wid : natlt (bm / (wm * tm) * (bn / (wn * tn))))
-  (lane : natlt warp_size)
-  (rD : chest2 real (wm * tm) (wn * tn))
-  (idx : natlt (wm * wn))
-  : slprop
-= exists* (eD : chest2 et tm tn).
-    own_lane_cells
-      (output_fragment gD bm bn tm tn wm wn
-        bid wid (idx / wn) (idx % wn))
-      eD lane **
-    pure (eD %~ ematrix_subtile rD tm tn (idx / wn) (idx % wn))
-
-let if_else_ (b : bool) (p q : slprop) : slprop =
-  if_ b p ** if_ (not b) q
-
-
-  ghost
-  fn forevery_extract_replace_eqtype
-    (#a : eqtype)
-    (z : a)
-    (p1 p2 : a -> slprop)
-    (#_ : squash (forall x. x =!= z ==> p1 x == p2 x))
-    requires forall+ (x : a). p1 x
-    ensures
-      p1 z **
-      (p2 z @==> forall+ (x : a). p2 x)
-  {
-    forevery_extract_if_eqtype z p1;
-    intro_trade #emp_inames
-      (p2 z)
-      (forall+ (x : a). p2 x)
-      (forall+ (x : a). if x = z then emp else p1 x)
-      fn _ {
-        forevery_map #a
-          (fun x -> if x = z then emp else p1 x)
-          (fun x -> if x = z then emp else p2 x)
-          fn x {
-            let is_z = x = z;
-            if is_z {
-              rewrite
-                (if x = z then emp else p1 x)
-              as emp;
-              rewrite emp as
-                (if x = z then emp else p2 x);
-            } else {
-              rewrite
-                (if x = z then emp else p1 x)
-              as p1 x;
-              rewrite p1 x as p2 x;
-              rewrite p2 x as
-                (if x = z then emp else p2 x);
-            }
-          };
-        forevery_unextract_if_eqtype z p2;
-      };
-  }
-
-  ghost
-  fn forevery_insert_replace_eqtype
-    (#a : eqtype)
-    (z : a)
-    (p1 p2 : a -> slprop)
-    (#_ : squash (forall x. x =!= z ==> p1 x == p2 x))
-    requires
-      p2 z **
-      (forall+ (x : a { x =!= z }). p1 x)
-    ensures forall+ (x : a). p2 x
-  {
-    forevery_map
-      #(x : a { x =!= z })
-      p1 p2
-      fn x {
-        rewrite p1 x as p2 x;
-      };
-    forevery_insert
-      #a
-      #(fun x -> x =!= z)
-      p2 z;
-    forevery_refine_ext
-      #a
-      #(fun x -> x =!= z \/ z == x)
-      (fun _ -> True)
-      p2;
-  }
-
-  let output_fragment_state_at
-    (#et : Type0) {| scalar et, real_like et |}
-    (#m #n : nat)
-    (gD : array2 et (rm m n))
-    (bm bn tm tn wm wn : pos)
-    (#_ : squash (bm /?+ m /\ bn /?+ n /\
-                  wm * tm /?+ bm /\ wn * tn /?+ bn))
-    (bid : natlt (m / bm * (n / bn)))
-    (wid : natlt (bm / (wm * tm) * (bn / (wn * tn))))
-    (lane : natlt warp_size)
-    (rD : chest2 real (wm * tm) (wn * tn))
-    (done : natle (wm * wn))
-    (idx : natlt (wm * wn))
-    : slprop
-  = if_else_ (idx < done)
-      (output_fragment_post
-        gD bm bn tm tn wm wn bid wid lane rD idx)
-      (live_lane_cells
-        (output_fragment gD bm bn tm tn wm wn
-          bid wid (idx / wn) (idx % wn))
-        lane)
-
-  let output_epilogue_state
-  (#et : Type0) {| scalar et, real_like et |}
-  (#m #n : nat)
-  (gD : array2 et (rm m n))
-  (bm bn tm tn wm wn : pos)
-  (#_ : squash (bm /?+ m /\ bn /?+ n /\
-                wm * tm /?+ bm /\ wn * tn /?+ bn))
-  (bid : natlt (m / bm * (n / bn)))
-  (wid : natlt (bm / (wm * tm) * (bn / (wn * tn))))
-  (lane : natlt warp_size)
-  (rD : chest2 real (wm * tm) (wn * tn))
-  (done : natle (wm * wn))
-  : slprop
-= forall+ (idx : natlt (wm * wn)).
-    output_fragment_state_at
-      gD bm bn tm tn wm wn bid wid lane rD done idx
-
-ghost
-fn output_epilogue_extract_step
-  (#et : Type0) {| scalar et, real_like et |}
-  (#m #n : nat)
-  (gD : array2 et (rm m n))
-  (bm bn tm tn wm wn : pos)
-  (#_ : squash (bm /?+ m /\ bn /?+ n /\
-                wm * tm /?+ bm /\ wn * tn /?+ bn))
-  (bid : natlt (m / bm * (n / bn)))
-  (wid : natlt (bm / (wm * tm) * (bn / (wn * tn))))
-  (lane : natlt warp_size)
-  (rD : chest2 real (wm * tm) (wn * tn))
-  (idx_ref : ref (szle (wm * wn)))
-  (done : szle (wm * wn) { SZ.v done < wm * wn })
-  preserves idx_ref |-> done
-  requires
-    output_epilogue_state
-      gD bm bn tm tn wm wn bid wid lane rD (SZ.v done)
-  ensures
-    output_fragment_state_at
-      gD bm bn tm tn wm wn bid wid lane rD
-      (SZ.v done) (SZ.v done) **
-    (output_fragment_state_at
-        gD bm bn tm tn wm wn bid wid lane rD
-        (SZ.v done + 1) (SZ.v done)
-      @==>
-      forall+ (idx : natlt (wm * wn)).
-        output_fragment_state_at
-          gD bm bn tm tn wm wn bid wid lane rD (SZ.v done + 1) idx)
-{
-  unfold output_epilogue_state
-    gD bm bn tm tn wm wn bid wid lane rD (SZ.v done);
-  forevery_extract_replace_eqtype
-    #(natlt (wm * wn))
-    (SZ.v done)
-    (output_fragment_state_at
-      gD bm bn tm tn wm wn bid wid lane rD (SZ.v done))
-    (output_fragment_state_at
-      gD bm bn tm tn wm wn bid wid lane rD (SZ.v done + 1));
-}
+open Kuiper.Kernel.GEMM.TensorCore2D.To.KernelDesc.Epilogue
+open Kuiper.Kernel.GEMM.TensorCore2D.To.EpilogueState
+open Kuiper.Kernel.GEMM.TensorCore2D.To.EpilogueLoopStep
 
 inline_for_extraction noextract
 fn epilogue_to
@@ -213,44 +41,69 @@ fn epilogue_to
   (#fC : perm)
   (#eC : chest2 et_cd m n)
   (#rC : chest2 real m n)
-  (#_ : squash (eC %~ rC))
   (gD : array2 et_cd (rm m n))
-  (#_ : squash (SZ.fits (m * n)))
-  (bm bn bk tm tn tk wm wn nthr : szp{
-    constraints bm bn bk tm tn tk wm wn /\
-    SZ.v nthr == bm / (wm * tm) * (bn / (wn * tn)) * warp_size})
-  (#_ : squash (bm /?+ m /\ bn /?+ n))
-  (#_ : squash (SZ.fits (bm * bk) /\ SZ.fits (bk * bn)))
-  (#_ : squash (SZ.fits (wm * wn)))
-  (#_ : squash (SZ.fits ((nthr / warp_size) * tm * tn)))
-  (#_ : squash (SZ.fits (tm * tn + warp_size)))
-  (sh : c_shmems (shmems_desc_to et_ab et_acc bm bn bk tm tn nthr))
-  (accFrags : array (fragment et_acc FragAcc tm tn tk FragLAcc))
-  (rAcc : chest2 real (wm * tm) (wn * tn))
-  (bid : szlt (m / bm * (n / bn)))
-  (tid : szlt nthr)
-  (#_ : squash (Pulse.Lib.Array.length accFrags == wm * wn))
-  preserves
-    gpu **
-    thread_id nthr tid **
-    gC |-> Frac fC eC **
-    fragarrayAcc_approximates wm wn accFrags rAcc
+  (d : epilogue_dims m n)
+  (sh : c_shmems
+    (shmems_desc_to et_ab et_acc d.bm d.bn d.bk d.tm d.tn d.nthr))
+  (accFrags : array
+    (fragment et_acc FragAcc d.tm d.tn d.tk FragLAcc))
+  (rAcc : chest2 real (d.wm * d.tm) (d.wn * d.tn))
+  (bid : szlt (m / d.bm * (n / d.bn)))
+  (tid : szlt d.nthr)
+  (#_ : squash (Pulse.Lib.Array.length accFrags == d.wm * d.wn))
+  norewrite
   requires
-    scratch_tile_live bm bn bk tm tn nthr sh tid **
-    output_lane_live gD bm bn tm tn wm wn bid tid
+    epilogue_frame #et_ab #et_cd #et_acc
+      #_ #_ #_ #_ #_
+      #m #n gC fC eC rC
+      d.bm d.bn d.bk d.tm d.tn d.tk d.wm d.wn d.nthr
+      sh accFrags rAcc tid **
+    output_lane_live gD d.bm d.bn d.tm d.tn d.wm d.wn bid tid
   ensures
-    scratch_tile_live bm bn bk tm tn nthr sh tid **
+    epilogue_frame #et_ab #et_cd #et_acc
+      #_ #_ #_ #_ #_
+      #m #n gC fC eC rC
+      d.bm d.bn d.bk d.tm d.tn d.tk d.wm d.wn d.nthr
+      sh accFrags rAcc tid **
     output_lane_approximates
-      gD bm bn tm tn wm wn bid tid
+      gD d.bm d.bn d.tm d.tn d.wm d.wn bid tid
       (chest_comb comb_r
         (ematrix_subtile
-          (ematrix_subtile rC bm bn
-            (bid / (n / bn)) (bid % (n / bn)))
-          (wm * tm) (wn * tn)
-          ((tid / warp_size) / (bn / (wn * tn)))
-          ((tid / warp_size) % (bn / (wn * tn))))
+          (ematrix_subtile rC d.bm d.bn
+            (bid / (n / d.bn)) (bid % (n / d.bn)))
+          (d.wm * d.tm) (d.wn * d.tn)
+          ((tid / warp_size) / (d.bn / (d.wn * d.tn)))
+          ((tid / warp_size) % (d.bn / (d.wn * d.tn))))
         rAcc)
 {
+  let bm = d.bm;
+  let bn = d.bn;
+  let bk = d.bk;
+  let tm = d.tm;
+  let tn = d.tn;
+  let tk = d.tk;
+  let wm = d.wm;
+  let wn = d.wn;
+  let nthr = d.nthr;
+  rewrite each d.bm as bm;
+  rewrite each d.bn as bn;
+  rewrite each d.bk as bk;
+  rewrite each d.tm as tm;
+  rewrite each d.tn as tn;
+  rewrite each d.tk as tk;
+  rewrite each d.wm as wm;
+  rewrite each d.wn as wn;
+  rewrite each d.nthr as nthr;
+  assert pure (constraints bm bn bk tm tn tk wm wn);
+  assert pure (bm /?+ m /\ bn /?+ n);
+  assert pure (SZ.fits (bm * bk) /\ SZ.fits (bk * bn));
+  assert pure (SZ.fits (wm * wn));
+  assert pure (SZ.fits ((nthr / warp_size) * tm * tn));
+  assert pure (SZ.fits (tm * tn + warp_size));
+  unfold epilogue_frame #et_ab #et_cd #et_acc
+    #_ #_ #_ #_ #_
+    #m #n gC fC eC rC
+    bm bn bk tm tn tk wm wn nthr sh accFrags rAcc tid;
   let wid = tid /^ warp_size;
   let lane = tid %^ warp_size;
   let mrow = bid /^ (n /^ bn);
@@ -334,152 +187,36 @@ fn epilogue_to
   fold output_epilogue_state
     gD bm bn tm tn wm wn bid wid lane
     (chest_comb comb_r rCWarp rAcc) 0;
-
-  with eScratch.
-    unfold scratch_tile_live bm bn bk tm tn nthr sh tid;
-  let sTile = scratch_tile_st bm bn bk tm tn nthr sh wid;
+  fold epilogue_frame #et_ab #et_cd #et_acc
+    #_ #_ #_ #_ #_
+    #m #n gC fC eC rC
+    bm bn bk tm tn tk wm wn nthr sh accFrags rAcc tid;
 
   let mut idx : szle (wm * wn) = 0sz;
   while (!idx <^ wm *^ wn)
     invariant live idx
     invariant
-      exists* (eScratchLoop : chest2 et_acc tm tn).
-        scratch_tile bm bn bk tm tn nthr sh
-          (SZ.v tid / warp_size)
-          |-> Frac (1.0R /. warp_size) eScratchLoop
+      epilogue_frame #et_ab #et_cd #et_acc
+        #_ #_ #_ #_ #_
+        #m #n gC fC eC rC
+        bm bn bk tm tn tk wm wn nthr
+        sh accFrags rAcc tid
     invariant
       output_epilogue_state
         gD bm bn tm tn wm wn bid wid lane
         (chest_comb comb_r rCWarp rAcc) !idx
-    invariant
-      fragarrayAcc_approximates wm wn accFrags rAcc
     decreases (wm * wn - !idx)
   {
-    with vidx. assert idx |-> vidx;
-    output_epilogue_extract_step
-      gD bm bn tm tn wm wn bid wid lane
-      (chest_comb comb_r rCWarp rAcc) idx vidx;
-    unfold output_fragment_state_at
-      gD bm bn tm tn wm wn bid wid lane
-      (chest_comb comb_r rCWarp rAcc) (SZ.v vidx) (SZ.v vidx);
-    unfold if_else_ (SZ.v vidx < SZ.v vidx)
-      (output_fragment_post
-        gD bm bn tm tn wm wn bid wid lane
-        (chest_comb comb_r rCWarp rAcc) (SZ.v vidx))
-      (live_lane_cells
-        (output_fragment gD bm bn tm tn wm wn
-          bid wid (SZ.v vidx / wn) (SZ.v vidx % wn))
-        lane);
-    Kuiper.Conditional.if_rewrite_bool
-      (SZ.v vidx < SZ.v vidx) false
-      (output_fragment_post
-        gD bm bn tm tn wm wn bid wid lane
-        (chest_comb comb_r rCWarp rAcc) (SZ.v vidx));
-    Kuiper.Conditional.if_elim_false
-      (output_fragment_post
-        gD bm bn tm tn wm wn bid wid lane
-        (chest_comb comb_r rCWarp rAcc) (SZ.v vidx));
-    Kuiper.Conditional.if_rewrite_bool
-      (not (SZ.v vidx < SZ.v vidx)) true
-      (live_lane_cells
-        (output_fragment gD bm bn tm tn wm wn
-          bid wid (SZ.v vidx / wn) (SZ.v vidx % wn))
-        lane);
-    Kuiper.Conditional.if_elim_true
-      (live_lane_cells
-        (output_fragment gD bm bn tm tn wm wn
-          bid wid (SZ.v vidx / wn) (SZ.v vidx % wn))
-        lane);
-
-    unfold fragarrayAcc_approximates wm wn accFrags rAcc;
-    with eAccFrags. assert accFrags `array_fragment_pts_to` eAccFrags;
-    array_fragment_pts_to_ref accFrags;
-    array_fragment_extract_ro accFrags vidx;
-
-    rewrite each
-      scratch_tile bm bn bk tm tn nthr sh (SZ.v tid / warp_size)
-    as sTile;
-    mma_store accFrags.(!idx) sTile;
-
-    let rCFrag =
-      ematrix_subtile rCWarp tm tn (SZ.v vidx / wn) (SZ.v vidx % wn);
-    let rAccFrag =
-      ematrix_subtile rAcc tm tn (SZ.v vidx / wn) (SZ.v vidx % wn);
-
-    assert pure (Seq.Base.index eAccFrags vidx %~ rAccFrag);
-    epilogue_fragment_from_warp comb comb_r gC
-      bm bn tm tn wm wn mrow mcol warpRow warpCol bid wid
-      #_ #_ #_ #rC #_
-      sTile #(Seq.Base.index eAccFrags vidx) #rAccFrag #_
-      gD !idx lane;
-    rewrite each sTile as
-      scratch_tile bm bn bk tm tn nthr sh (SZ.v tid / warp_size);
-
-    with eOut.
-      assert own_lane_cells
-        (output_fragment gD bm bn tm tn wm wn
-          bid wid (SZ.v vidx / wn) (SZ.v vidx % wn))
-        eOut lane;
-    fold output_fragment_post
-      gD bm bn tm tn wm wn bid wid lane
-      (chest_comb comb_r rCWarp rAcc) vidx;
-    Kuiper.Conditional.if_intro_true
-      (output_fragment_post
-        gD bm bn tm tn wm wn bid wid lane
-        (chest_comb comb_r rCWarp rAcc) (SZ.v vidx));
-    Kuiper.Conditional.if_rewrite_bool
-      true (SZ.v vidx < SZ.v vidx + 1)
-      (output_fragment_post
-        gD bm bn tm tn wm wn bid wid lane
-        (chest_comb comb_r rCWarp rAcc) (SZ.v vidx));
-    Kuiper.Conditional.if_intro_false
-      (live_lane_cells
-        (output_fragment gD bm bn tm tn wm wn
-          bid wid (SZ.v vidx / wn) (SZ.v vidx % wn))
-        lane);
-    Kuiper.Conditional.if_rewrite_bool
-      false (not (SZ.v vidx < SZ.v vidx + 1))
-      (live_lane_cells
-        (output_fragment gD bm bn tm tn wm wn
-          bid wid (SZ.v vidx / wn) (SZ.v vidx % wn))
-        lane);
-    fold if_else_ (SZ.v vidx < SZ.v vidx + 1)
-      (output_fragment_post
-        gD bm bn tm tn wm wn bid wid lane
-        (chest_comb comb_r rCWarp rAcc) (SZ.v vidx))
-      (live_lane_cells
-        (output_fragment gD bm bn tm tn wm wn
-          bid wid (SZ.v vidx / wn) (SZ.v vidx % wn))
-        lane);
-    fold output_fragment_state_at
-      gD bm bn tm tn wm wn bid wid lane
-      (chest_comb comb_r rCWarp rAcc)
-      (SZ.v vidx + 1) (SZ.v vidx);
-    Pulse.Lib.Trade.elim_trade
-      (output_fragment_state_at
-        gD bm bn tm tn wm wn bid wid lane
-        (chest_comb comb_r rCWarp rAcc)
-        (SZ.v vidx + 1) (SZ.v vidx))
-      (forall+ (fi : natlt (wm * wn)).
-        output_fragment_state_at
-          gD bm bn tm tn wm wn bid wid lane
-          (chest_comb comb_r rCWarp rAcc) (SZ.v vidx + 1) fi);
-    ambig_trade_elim ();
-    fold fragarrayAcc_approximates wm wn accFrags rAcc;
-
-    fold output_epilogue_state
-      gD bm bn tm tn wm wn bid wid lane
-      (chest_comb comb_r rCWarp rAcc) (SZ.v vidx + 1);
-    with vnext. assert idx |-> vnext;
-    idx := sz_succ !idx;
-    rewrite each
-      (SZ.v vnext + 1)
-    as
-      (SZ.v (sz_succ vnext));
+    let before = !idx;
+    epilogue_loop_step comb comb_r gC gD
+      bm bn bk tm tn tk wm wn nthr
+      sh accFrags rAcc bid tid wid lane rCWarp idx before;
+    let next = !idx;
+    assert pure (SZ.v next == SZ.v before + 1);
+    rewrite each (SZ.v before + 1) as (SZ.v next);
   };
 
   rewrite each !idx as (wm *^ wn);
-  fold scratch_tile_live bm bn bk tm tn nthr sh tid;
   unfold output_epilogue_state
     gD bm bn tm tn wm wn bid wid lane
     (chest_comb comb_r rCWarp rAcc) (wm * wn);
@@ -608,4 +345,36 @@ fn epilogue_to
         ((tid / warp_size) / (bn / (wn * tn)))
         ((tid / warp_size) % (bn / (wn * tn))))
       rAcc);
+  rewrite
+    epilogue_frame #et_ab #et_cd #et_acc
+      #_ #_ #_ #_ #_
+      #m #n gC fC eC rC
+      bm bn bk tm tn tk wm wn nthr sh accFrags rAcc tid
+  as
+    epilogue_frame #et_ab #et_cd #et_acc
+      #_ #_ #_ #_ #_
+      #m #n gC fC eC rC
+      d.bm d.bn d.bk d.tm d.tn d.tk d.wm d.wn d.nthr
+      sh accFrags rAcc tid;
+  rewrite
+    output_lane_approximates gD bm bn tm tn wm wn bid tid
+      (chest_comb comb_r
+        (ematrix_subtile
+          (ematrix_subtile rC bm bn
+            (bid / (n / bn)) (bid % (n / bn)))
+          (wm * tm) (wn * tn)
+          ((tid / warp_size) / (bn / (wn * tn)))
+          ((tid / warp_size) % (bn / (wn * tn))))
+        rAcc)
+  as
+    output_lane_approximates gD
+      d.bm d.bn d.tm d.tn d.wm d.wn bid tid
+      (chest_comb comb_r
+        (ematrix_subtile
+          (ematrix_subtile rC d.bm d.bn
+            (bid / (n / d.bn)) (bid % (n / d.bn)))
+          (d.wm * d.tm) (d.wn * d.tn)
+          ((tid / warp_size) / (d.bn / (d.wn * d.tn)))
+          ((tid / warp_size) % (d.bn / (d.wn * d.tn))))
+        rAcc);
 }
