src/lib/kernel/gemm/Kuiper.Kernel.GEMM.TensorCore2D.To.Finish.fst
@@ -1,0 +1,173 @@
+module Kuiper.Kernel.GEMM.TensorCore2D.To.Finish
+
+#lang-pulse
+
+open Kuiper
+#set-options "--ifuel 1 --initial_fuel 0 --max_fuel 1"
+#set-options "--z3rlimit 15"
+
+open Kuiper.Array.Vectorized { has_vec_cpy, chunk }
+open Kuiper.EMatrix
+open Kuiper.EMatrix.Tiling
+open Kuiper.Tensor
+open Kuiper.Array2.Strided
+open Kuiper.Tensor.Tiling
+open Kuiper.Tensor.Layout.Alg { l2_row_major as rm }
+open Kuiper.Spec.GEMM
+open Kuiper.TensorCore
+open Pulse.Lib.Array
+
+module SZ = Kuiper.SizeT
+module FB = Kuiper.Kernel.GEMM.FlipFlopBarrier2
+module MS = Kuiper.Spec.GEMM
+
+open Kuiper.Kernel.GEMM.TensorCore2D.KernelDesc
+open Kuiper.Kernel.GEMM.TensorCore2D.To.KernelDesc
+open Kuiper.Kernel.GEMM.TensorCore2D.To.Epilogue
+open Kuiper.Kernel.GEMM.TensorCore2D.To.EpilogueState
+open Kuiper.Kernel.GEMM.TensorCore2D.To.OutputProof
+open Kuiper.Kernel.GEMM.TensorCore2D.To.Cleanup
+
+inline_for_extraction noextract
+fn finish
+  (#et_ab #et_cd #et_acc : Type0)
+  {| scalar et_ab, has_vec_cpy et_ab, scalar et_cd, real_like et_cd,
+     scalar et_acc, real_like et_acc |}
+  (comb : et_cd -> et_acc -> et_cd)
+  (comb_r : binop real { approx2 comb comb_r })
+  (#m #n #k : szp)
+  (gC : array2 et_cd (rm m n))
+  (#eC : chest2 et_cd m n)
+  (gD : array2 et_cd (rm m n))
+  (bm bn bk tm tn tk wm wn : szp {
+    constraints bm bn bk tm tn tk wm wn })
+  (#tiles_div : squash (bm /?+ m /\ bn /?+ n))
+  (#_ : squash (wm * tm /?+ m /\ wn * tn /?+ n))
+  (#shared_fits : squash (SZ.fits (bm * bk) /\ SZ.fits (bk * bn)))
+  (#output_fits : squash (SZ.fits (m * n)))
+  (#fragment_fits : squash (SZ.fits (tm * tn + warp_size)))
+  (#tile_count_fits : squash (SZ.fits (wm * wn)))
+  (#fC : perm)
+  (rA : chest2 real m k)
+  (rB : chest2 real k n)
+  (rC : chest2 real m n)
+  (nthr : szp {
+    SZ.v nthr == bm / (wm * tm) * (bn / (wn * tn)) * warp_size})
+  (#scratch_fits : squash (SZ.fits ((nthr / warp_size) * tm * tn)))
+  (sh : c_shmems (shmems_desc_to et_ab et_acc bm bn bk tm tn nthr))
+  (sA : array2 et_ab (rm bm bk) { core sA == fst sh })
+  (sB : array2 et_ab (rm bk bn) { core sB == fst (snd sh) })
+  (bid : szlt (m / bm * (n / bn)))
+  (tid : szlt nthr)
+  (mrow : szlt (m / bm))
+  (mcol : szlt (n / bn))
+  (wid : szlt (nthr / warp_size))
+  (warpRow : szlt (bm / (wm * tm)))
+  (warpCol : szlt (bn / (wn * tn)))
+  (#_ : squash (
+    SZ.v mrow == SZ.v bid / (SZ.v n / SZ.v bn) /\
+    SZ.v mcol == SZ.v bid % (SZ.v n / SZ.v bn) /\
+    SZ.v wid == SZ.v tid / warp_size /\
+    SZ.v warpRow == SZ.v wid / (SZ.v bn / (SZ.v wn * SZ.v tn)) /\
+    SZ.v warpCol == SZ.v wid % (SZ.v bn / (SZ.v wn * SZ.v tn))))
+  (gwRow : enatlt (m / (wm * tm)) {
+    gwRow == mrow * (bm / (wm * tm)) + warpRow })
+  (gwCol : enatlt (n / (wn * tn)) {
+    gwCol == mcol * (bn / (wn * tn)) + warpCol })
+  (accFrags : array (fragment et_acc FragAcc tm tn tk FragLAcc))
+  (#acc_length : squash (Pulse.Lib.Array.length accFrags == wm * wn))
+  (rAcc : chest2 real (wm * tm) (wn * tn) {
+    rAcc == MS.matmul
+      (ematrix_subtile rA (wm * tm) k
+        (warp_tile_i #m #n bm bn bk tm tn tk wm wn
+          nthr bid (tid / warp_size)) 0)
+      (ematrix_subtile rB k (wn * tn) 0
+        (warp_tile_j #m #n bm bn bk tm tn tk wm wn
+          nthr bid (tid / warp_size))) })
+  requires
+    epilogue_frame #et_ab #et_cd #et_acc
+      #_ #_ #_ #_ #_
+      #m #n gC (fC /. (m / bm * (n / bn) * nthr)) eC rC
+      bm bn bk tm tn tk wm wn nthr sh accFrags rAcc tid **
+    output_lane_live gD bm bn tm tn wm wn bid tid **
+    (exists* em1. FB.bp_sharing sA em1 nthr) **
+    (exists* em2. FB.bp_sharing sB em2 nthr)
+  ensures
+    pure (eC %~ rC) **
+    gpu **
+    thread_id nthr tid **
+    gC |-> Frac (fC /. (m / bm * (n / bn) * nthr)) eC **
+    shared_thread_live bm bn bk tm tn nthr sh tid **
+    output_lane_approximates gD bm bn tm tn wm wn bid tid
+      (ematrix_subtile
+        (ematrix_subtile (MS.mmcomb comb_r rC rA rB)
+          bm bn mrow mcol)
+        (wm * tm) (wn * tn) warpRow warpCol)
+{
+  let dims : epilogue_dims m n = {
+    bm; bn; bk; tm; tn; tk; wm; wn; nthr;
+    tiles_div; shared_fits; output_fits; tile_count_fits;
+    scratch_fits; fragment_fits;
+  };
+  rewrite
+    epilogue_frame #et_ab #et_cd #et_acc
+      #_ #_ #_ #_ #_
+      #m #n gC (fC /. (m / bm * (n / bn) * nthr)) eC rC
+      bm bn bk tm tn tk wm wn nthr sh accFrags rAcc tid
+  as
+    epilogue_frame #et_ab #et_cd #et_acc
+      #_ #_ #_ #_ #_
+      #m #n gC (fC /. (m / bm * (n / bn) * nthr)) eC rC
+      dims.bm dims.bn dims.bk dims.tm dims.tn dims.tk
+      dims.wm dims.wn dims.nthr sh accFrags rAcc tid;
+  rewrite
+    output_lane_live gD bm bn tm tn wm wn bid tid
+  as
+    output_lane_live gD
+      dims.bm dims.bn dims.tm dims.tn dims.wm dims.wn bid tid;
+  epilogue_to #et_ab #et_cd #et_acc comb comb_r #m #n
+    gC #(fC /. (m / bm * (n / bn) * nthr)) #eC #rC
+    gD dims
+    sh accFrags rAcc bid tid #acc_length;
+  rewrite
+    epilogue_frame #et_ab #et_cd #et_acc
+      #_ #_ #_ #_ #_
+      #m #n gC (fC /. (m / bm * (n / bn) * nthr)) eC rC
+      dims.bm dims.bn dims.bk dims.tm dims.tn dims.tk
+      dims.wm dims.wn dims.nthr sh accFrags rAcc tid
+  as
+    epilogue_frame #et_ab #et_cd #et_acc
+      #_ #_ #_ #_ #_
+      #m #n gC (fC /. (m / bm * (n / bn) * nthr)) eC rC
+      bm bn bk tm tn tk wm wn nthr sh accFrags rAcc tid;
+  rewrite
+    output_lane_approximates gD
+      dims.bm dims.bn dims.tm dims.tn dims.wm dims.wn bid tid
+      (chest_comb comb_r
+        (ematrix_subtile
+          (ematrix_subtile rC dims.bm dims.bn
+            (bid / (n / dims.bn)) (bid % (n / dims.bn)))
+          (dims.wm * dims.tm) (dims.wn * dims.tn)
+          ((tid / warp_size) / (dims.bn / (dims.wn * dims.tn)))
+          ((tid / warp_size) % (dims.bn / (dims.wn * dims.tn))))
+        rAcc)
+  as
+    output_lane_approximates gD bm bn tm tn wm wn bid tid
+      (chest_comb comb_r
+        (ematrix_subtile
+          (ematrix_subtile rC bm bn
+            (bid / (n / bn)) (bid % (n / bn)))
+          (wm * tm) (wn * tn)
+          ((tid / warp_size) / (bn / (wn * tn)))
+          ((tid / warp_size) % (bn / (wn * tn))))
+        rAcc);
+  unfold epilogue_frame #et_ab #et_cd #et_acc
+    #_ #_ #_ #_ #_
+    #m #n gC (fC /. (m / bm * (n / bn) * nthr)) eC rC
+    bm bn bk tm tn tk wm wn nthr sh accFrags rAcc tid;
+  normalize_output comb_r gD
+    bm bn bk tm tn tk wm wn rA rB rC nthr
+    bid tid mrow mcol wid warpRow warpCol gwRow gwCol rAcc;
+  cleanup #et_ab #et_acc
+    bm bn bk tm tn tk wm wn nthr sh sA sB tid accFrags rAcc;
+}
