src/lib/kernel/gemm/Kuiper.Kernel.GEMM.TensorCore2D.To.KLoopState.fsti
@@ -1,0 +1,24 @@
+module Kuiper.Kernel.GEMM.TensorCore2D.To.KLoopState
+
+open Kuiper
+
+module SZ = Kuiper.SizeT
+
+open Kuiper.EMatrix
+open Kuiper.Spec.GEMM
+
+let barrier_iteration (v : SZ.t) : nat = 2 * SZ.v v
+
+let tile_barrier_iteration (k bk : szp) : nat =
+  2 * (SZ.v k / SZ.v bk)
+
+let tiled_partial_matmul
+  (#rows #shared #cols #tm #tk #tn : nat)
+  (z : chest2 real tm tn)
+  (a : chest2 (chest2 real tm tk) rows shared)
+  (b : chest2 (chest2 real tk tn) shared cols)
+  (row : natlt rows)
+  (col : natlt cols)
+  (upto : nat { upto <= shared })
+  : chest2 real tm tn
+= __gmatmul_single z matmul matplus a b row col upto
