src/lib/kernel/gemm/Kuiper.Kernel.GEMM.TensorCore2D.To.KernelDesc.TeardownOutput.fst
@@ -1,0 +1,188 @@
+module Kuiper.Kernel.GEMM.TensorCore2D.To.KernelDesc.TeardownOutput
+
+#lang-pulse
+
+open Kuiper
+#set-options "--ifuel 1 --initial_fuel 0 --max_fuel 1 --z3rlimit 15"
+
+open Kuiper.EMatrix
+open Kuiper.EMatrix.Tiling
+open Kuiper.Tensor
+open Kuiper.Tensor.Tiling
+open Kuiper.Tensor.Layout.Alg { l2_row_major as rm }
+open Kuiper.Kernel.GEMM.Tiled.Common.Vec
+
+module SZ = Kuiper.SizeT
+module MS = Kuiper.Spec.GEMM
+
+open Kuiper.Kernel.GEMM.TensorCore2D.KernelDesc
+open Kuiper.Kernel.GEMM.TensorCore2D.To.KernelDesc
+open Kuiper.Kernel.GEMM.TensorCore2D.To.KernelDesc.TeardownHelpers
+open Kuiper.Kernel.GEMM.TensorCore2D.To.KernelDesc.TeardownWarp
+open Kuiper.Kernel.GEMM.TensorCore2D.To.KernelDesc.TeardownBlock
+
+ghost
+fn gather_output
+  (#et_cd : Type0) {| scalar et_cd, real_like et_cd |}
+  (comb_r : binop real)
+  (#m #n #k : szp)
+  (gD : array2 et_cd (rm m n))
+  (bm bn bk tm tn tk wm wn : szp {
+    constraints bm bn bk tm tn tk wm wn })
+  (#_ : squash (bm /?+ m /\ bn /?+ n))
+  (#_ : squash (wm * tm /?+ bm /\ wn * tn /?+ bn))
+  (#_ : squash (tm /?+ (wm * tm) /\ tn /?+ (wn * tn)))
+  (nblk : szp { SZ.v nblk == m / bm * (n / bn) })
+  (nthr : szp {
+    SZ.v nthr == bm / (wm * tm) * (bn / (wn * tn)) * warp_size })
+  (rA : chest2 real m k)
+  (rB : chest2 real k n)
+  (rC : chest2 real m n)
+  ()
+  norewrite
+  requires
+    (forall+ (bid : natlt nblk) (tid : natlt nthr).
+      output_lane_approximates gD bm bn tm tn wm wn bid tid
+        (ematrix_subtile
+          (ematrix_subtile (MS.mmcomb comb_r rC rA rB)
+            bm bn (bid / (n / bn)) (bid % (n / bn)))
+          (wm * tm) (wn * tn)
+          ((tid / warp_size) / (bn / (wn * tn)))
+          ((tid / warp_size) % (bn / (wn * tn))))) **
+    pure (SZ.fits ((rm m n).ulen))
+  ensures
+    exists* (eD : chest2 et_cd m n).
+      gD |-> eD ** pure (eD %~ MS.mmcomb comb_r rC rA rB)
+{
+  forevery_map
+    (fun (bid : natlt nblk) ->
+      forall+ (tid : natlt nthr).
+        output_lane_approximates gD bm bn tm tn wm wn bid tid
+          (ematrix_subtile
+            (ematrix_subtile (MS.mmcomb comb_r rC rA rB)
+              bm bn (bid / (n / bn)) (bid % (n / bn)))
+            (wm * tm) (wn * tn)
+            ((tid / warp_size) / (bn / (wn * tn)))
+            ((tid / warp_size) % (bn / (wn * tn)))))
+    (fun (bid : natlt nblk) ->
+      exists* (eBlock : chest2 et_cd bm bn).
+        block_tile gD (SZ.v bm) (SZ.v bn) bid |-> eBlock **
+        pure (eBlock %~
+          ematrix_subtile (MS.mmcomb comb_r rC rA rB)
+            bm bn (bid / (n / bn)) (bid % (n / bn))))
+    fn bid {
+      forevery_ext
+        (fun (tid : natlt nthr) ->
+          output_lane_approximates gD bm bn tm tn wm wn bid tid
+            (ematrix_subtile
+              (ematrix_subtile (MS.mmcomb comb_r rC rA rB)
+                bm bn (bid / (n / bn)) (bid % (n / bn)))
+              (wm * tm) (wn * tn)
+              ((tid / warp_size) / (bn / (wn * tn)))
+              ((tid / warp_size) % (bn / (wn * tn)))))
+        (fun (tid : natlt nthr) ->
+          output_lane_approximates gD bm bn tm tn wm wn bid
+            ((tid / warp_size) * warp_size + tid % warp_size)
+            (ematrix_subtile
+              (ematrix_subtile (MS.mmcomb comb_r rC rA rB)
+                bm bn (bid / (n / bn)) (bid % (n / bn)))
+              (wm * tm) (wn * tn)
+              ((tid / warp_size) / (bn / (wn * tn)))
+              ((tid / warp_size) % (bn / (wn * tn)))));
+      forevery_factor' nthr (nthr / warp_size) warp_size
+        (fun wid lane ->
+          output_lane_approximates gD bm bn tm tn wm wn bid
+            (wid * warp_size + lane)
+            (ematrix_subtile
+              (ematrix_subtile (MS.mmcomb comb_r rC rA rB)
+                bm bn (bid / (n / bn)) (bid % (n / bn)))
+              (wm * tm) (wn * tn)
+              (wid / (bn / (wn * tn)))
+              (wid % (bn / (wn * tn)))));
+      forevery_map
+        (fun (wid : natlt (nthr / warp_size)) ->
+          forall+ (lane : natlt warp_size).
+            output_lane_approximates gD bm bn tm tn wm wn bid
+              (wid * warp_size + lane)
+              (ematrix_subtile
+                (ematrix_subtile (MS.mmcomb comb_r rC rA rB)
+                  bm bn (bid / (n / bn)) (bid % (n / bn)))
+                (wm * tm) (wn * tn)
+                (wid / (bn / (wn * tn)))
+                (wid % (bn / (wn * tn)))))
+        (fun (wid : natlt (nthr / warp_size)) ->
+          exists* (eWarp : chest2 et_cd (wm * tm) (wn * tn)).
+            warp_tile (block_tile gD (SZ.v bm) (SZ.v bn) bid)
+              (wm * tm) (wn * tn) wid |-> eWarp **
+            pure (eWarp %~
+              ematrix_subtile
+                (ematrix_subtile (MS.mmcomb comb_r rC rA rB)
+                  bm bn (bid / (n / bn)) (bid % (n / bn)))
+                (wm * tm) (wn * tn)
+                (wid / (bn / (wn * tn)))
+                (wid % (bn / (wn * tn)))))
+        fn wid {
+          gather_warp gD bm bn bk tm tn tk wm wn
+            nblk nthr bid wid
+            (ematrix_subtile
+              (ematrix_subtile (MS.mmcomb comb_r rC rA rB)
+                bm bn (bid / (n / bn)) (bid % (n / bn)))
+              (wm * tm) (wn * tn)
+              (wid / (bn / (wn * tn)))
+              (wid % (bn / (wn * tn))));
+        };
+      gather_block gD bm bn bk tm tn tk wm wn
+        nblk nthr bid
+        (ematrix_subtile (MS.mmcomb comb_r rC rA rB)
+          bm bn (bid / (n / bn)) (bid % (n / bn)));
+    };
+  forevery_map
+    #(natlt nblk)
+    (fun (bid : natlt nblk) ->
+      exists* (eBlock : chest2 et_cd bm bn).
+        block_tile gD (SZ.v bm) (SZ.v bn) bid |-> eBlock **
+        pure (eBlock %~
+          ematrix_subtile (MS.mmcomb comb_r rC rA rB)
+            bm bn (bid / (n / bn)) (bid % (n / bn))))
+    (fun (bid : natlt nblk) ->
+      exists* (eBlock : chest2 et_cd bm bn).
+        block_tile gD (SZ.v bm) (SZ.v bn)
+          ((bid / (n / bn)) * (n / bn) + bid % (n / bn)) |-> eBlock **
+        pure (eBlock %~
+          ematrix_subtile (MS.mmcomb comb_r rC rA rB)
+            bm bn (bid / (n / bn)) (bid % (n / bn))))
+    fn bid {
+      FStar.Math.Lemmas.euclidean_division_definition bid (n / bn);
+      rewrite each bid as
+        ((bid / (n / bn)) * (n / bn) + bid % (n / bn));
+    };
+  forevery_factor' nblk (m / bm) (n / bn)
+    (fun br bc ->
+      exists* (eBlock : chest2 et_cd bm bn).
+        block_tile gD (SZ.v bm) (SZ.v bn)
+          (br * (n / bn) + bc) |-> eBlock **
+        pure (eBlock %~
+          ematrix_subtile (MS.mmcomb comb_r rC rA rB) bm bn br bc));
+  forevery_map_2
+    #(natlt (m / bm)) #(natlt (n / bn))
+    (fun br bc ->
+      exists* (eBlock : chest2 et_cd bm bn).
+        block_tile gD (SZ.v bm) (SZ.v bn)
+          (br * (n / bn) + bc) |-> eBlock **
+        pure (eBlock %~
+          ematrix_subtile (MS.mmcomb comb_r rC rA rB) bm bn br bc))
+    (fun br bc ->
+      exists* (eBlock : chest2 et_cd bm bn).
+        array2_subtile gD (SZ.v bm) (SZ.v bn) br bc |-> eBlock **
+        pure (eBlock %~
+          ematrix_subtile (MS.mmcomb comb_r rC rA rB) bm bn br bc))
+    fn br bc {
+      assert pure ((br * (n / bn) + bc) / (n / bn) == br);
+      assert pure ((br * (n / bn) + bc) % (n / bn) == bc);
+      rewrite each block_tile gD (SZ.v bm) (SZ.v bn)
+        (br * (n / bn) + bc)
+      as array2_subtile gD (SZ.v bm) (SZ.v bn) br bc;
+    };
+  array2_untile_approximates gD (SZ.v bm) (SZ.v bn)
+    (MS.mmcomb comb_r rC rA rB);
+}
