src/lib/kernel/gemm/Kuiper.Kernel.GEMM.TensorCore2D.To.KernelDesc.TeardownWarp.fsti
@@ -1,0 +1,46 @@
+module Kuiper.Kernel.GEMM.TensorCore2D.To.KernelDesc.TeardownWarp
+
+#lang-pulse
+
+open Kuiper
+#set-options "--ifuel 1 --initial_fuel 0 --max_fuel 1 --z3rlimit 15"
+
+open Kuiper.EMatrix
+open Kuiper.EMatrix.Tiling
+open Kuiper.Tensor
+open Kuiper.Tensor.Tiling
+open Kuiper.Tensor.Layout.Alg { l2_row_major as rm }
+open Kuiper.Kernel.GEMM.Tiled.Common.Vec
+
+module SZ = Kuiper.SizeT
+
+open Kuiper.Kernel.GEMM.TensorCore2D.KernelDesc
+open Kuiper.Kernel.GEMM.TensorCore2D.To.KernelDesc
+
+ghost
+fn gather_warp
+  (#et_cd : Type0) {| scalar et_cd, real_like et_cd |}
+  (#m #n : szp)
+  (gD : array2 et_cd (rm m n))
+  (bm bn bk tm tn tk wm wn : szp {
+    constraints bm bn bk tm tn tk wm wn })
+  (#_ : squash (bm /?+ m /\ bn /?+ n))
+  (#_ : squash (wm * tm /?+ bm /\ wn * tn /?+ bn))
+  (#_ : squash (tm /?+ (wm * tm) /\ tn /?+ (wn * tn)))
+  (#_ : squash (SZ.fits ((rm m n).ulen)))
+  (nblk : szp { SZ.v nblk == m / bm * (n / bn) })
+  (nthr : szp {
+    SZ.v nthr == bm / (wm * tm) * (bn / (wn * tn)) * warp_size })
+  (bid : natlt nblk)
+  (wid : natlt (nthr / warp_size))
+  (rWarp : chest2 real (wm * tm) (wn * tn))
+  requires
+    forall+ (lane : natlt warp_size).
+      output_lane_approximates
+        gD bm bn tm tn wm wn bid (wid * warp_size + lane)
+        rWarp
+  ensures
+    exists* (eWarp : chest2 et_cd (wm * tm) (wn * tn)).
+      warp_tile (block_tile gD (SZ.v bm) (SZ.v bn) bid)
+        (wm * tm) (wn * tn) wid |-> eWarp **
+      pure (eWarp %~ rWarp)
