src/lib/kernel/gemm/Kuiper.Kernel.GEMM.TensorCore2D.To.OutputProof.fsti
@@ -1,0 +1,72 @@
+module Kuiper.Kernel.GEMM.TensorCore2D.To.OutputProof
+
+#lang-pulse
+
+open Kuiper
+open Kuiper.EMatrix
+open Kuiper.EMatrix.Tiling
+open Kuiper.Tensor
+open Kuiper.Tensor.Layout.Alg { l2_row_major as rm }
+
+module SZ = Kuiper.SizeT
+module MS = Kuiper.Spec.GEMM
+
+open Kuiper.Kernel.GEMM.TensorCore2D.KernelDesc
+open Kuiper.Kernel.GEMM.TensorCore2D.To.KernelDesc
+
+noextract
+ghost fn normalize_output
+  (#et_cd : Type0) {| scalar et_cd, real_like et_cd |}
+  (comb_r : binop real)
+  (#m #n #k : szp)
+  (gD : array2 et_cd (rm m n))
+  (bm bn bk tm tn tk wm wn : szp {
+    constraints bm bn bk tm tn tk wm wn })
+  (#_ : squash (bm /?+ m /\ bn /?+ n))
+  (#_ : squash (wm * tm /?+ m /\ wn * tn /?+ n))
+  (rA : chest2 real m k)
+  (rB : chest2 real k n)
+  (rC : chest2 real m n)
+  (nthr : szp {
+    SZ.v nthr == bm / (wm * tm) * (bn / (wn * tn)) * warp_size})
+  (bid : szlt (m / bm * (n / bn)))
+  (tid : szlt nthr)
+  (mrow : szlt (m / bm))
+  (mcol : szlt (n / bn))
+  (wid : szlt (nthr / warp_size))
+  (warpRow : szlt (bm / (wm * tm)))
+  (warpCol : szlt (bn / (wn * tn)))
+  (#_ : squash (
+    SZ.v mrow == SZ.v bid / (SZ.v n / SZ.v bn) /\
+    SZ.v mcol == SZ.v bid % (SZ.v n / SZ.v bn) /\
+    SZ.v wid == SZ.v tid / warp_size /\
+    SZ.v warpRow == SZ.v wid / (SZ.v bn / (SZ.v wn * SZ.v tn)) /\
+    SZ.v warpCol == SZ.v wid % (SZ.v bn / (SZ.v wn * SZ.v tn))))
+  (gwRow : enatlt (m / (wm * tm)) {
+    gwRow == mrow * (bm / (wm * tm)) + warpRow })
+  (gwCol : enatlt (n / (wn * tn)) {
+    gwCol == mcol * (bn / (wn * tn)) + warpCol })
+  (rAcc : chest2 real (wm * tm) (wn * tn) {
+    rAcc == MS.matmul
+      (ematrix_subtile rA (wm * tm) k
+        (warp_tile_i #m #n bm bn bk tm tn tk wm wn
+          nthr bid (tid / warp_size)) 0)
+      (ematrix_subtile rB k (wn * tn) 0
+        (warp_tile_j #m #n bm bn bk tm tn tk wm wn
+          nthr bid (tid / warp_size))) })
+  requires
+    output_lane_approximates gD bm bn tm tn wm wn bid tid
+      (chest_comb comb_r
+        (ematrix_subtile
+          (ematrix_subtile rC bm bn
+            (bid / (n / bn)) (bid % (n / bn)))
+          (wm * tm) (wn * tn)
+          ((tid / warp_size) / (bn / (wn * tn)))
+          ((tid / warp_size) % (bn / (wn * tn))))
+        rAcc)
+  ensures
+    output_lane_approximates gD bm bn tm tn wm wn bid tid
+      (ematrix_subtile
+        (ematrix_subtile (MS.mmcomb comb_r rC rA rB)
+          bm bn mrow mcol)
+        (wm * tm) (wn * tn) warpRow warpCol)
